BlasterBenchmarks/UPLC/Examples/Integer/Saturate.lean
@@ -12,6 +12,8 @@ open UPLC.Uplc
 
 /-! # Test cases with Valid result expected -/
 
+set_option warn.sorry false
+
 def saturate : Program :=
     Program.Program (Version.Version 1 1 0)
     (Term.Apply
