BlasterBenchmarks/UPLC/Examples/Integer/Subtract.lean
@@ -13,6 +13,7 @@ open UPLC.Uplc
 
 /-! # Test cases with Valid result expected -/
 
+set_option warn.sorry false
 def subtractInteger: Program :=
     (Program.Program (Version.Version 1 1 0)
     (Term.Lam "x"
