BlasterBenchmarks/UPLC/Examples/Onchain/ProcessSCOrder/STO14.lean
@@ -2,7 +2,6 @@ import BlasterBenchmarks.UPLC.Builtins
 import BlasterBenchmarks.UPLC.CekValue
 import BlasterBenchmarks.UPLC.Examples.Utils
 import BlasterBenchmarks.UPLC.Examples.Onchain.ProcessSCOrder.ProcessSCOrder
-import BlasterBenchmarks.UPLC.PreProcess
 import BlasterBenchmarks.UPLC.Uplc
 import Solver.Command.Tactic
 
@@ -11,21 +10,30 @@ open Tests.Uplc.Onchain
 
 set_option warn.sorry false
 -- STO14: Min Ratio Violation for Buying Stablecoin Order
+
+-- Provable once subgoal splitting supported inherently in blaster
 theorem sto14 :
   ∀ (x : ProcessSCInput),
   isBuySCOrder x →
   validOrderInput x →
-  isInvalidMinReserveStatus (fromHaltState $ prop_compiledProcessSCOrder x) →
+  isInvalidMinReserveStatus (fromHaltState $ appliedProcessSCOrder x) →
   validMinRatioViolation x := by sorry
-  -- intro x
-  -- blaster (only-optimize: 1)
-  -- by_cases x.state.crN_SC = 0
-  -- . blaster
-  -- . by_cases x.state.crN_RC = 0
-  --   . by_cases x.orderRate < mkRatio x.state.crReserve x.state.crN_SC <;> blaster
-  --   . blaster
 
--- NOTE: Remove solver options once subgoal splitting is supported
-#solve (timeout: 2) (solve-result: 2) [ sto14 ]
+-- Example of subgoal splitting to reduce complexity at Smt solver level
+theorem sto14_part1 :
+  ∀ (x : ProcessSCInput),
+  isBuySCOrder x →
+  validOrderInput x →
+  x.state.crN_SC = 0 →
+  isInvalidMinReserveStatus (fromHaltState $ appliedProcessSCOrder x) →
+  validMinRatioViolation x := by sorry
+
+theorem sto14_part2 :
+  ∀ (x : ProcessSCInput),
+  isBuySCOrder x →
+  validOrderInput x →
+  x.state.crN_SC ≠ 0 →
+  isInvalidMinReserveStatus (fromHaltState $ appliedProcessSCOrder x) →
+  validMinRatioViolation x := by sorry
 
 end Tests.Uplc.Onchain.ProcessSCOrder
