BlasterBenchmarks/UPLC/Examples/Onchain/ProcessSCOrder/STO1_5.lean
@@ -2,7 +2,6 @@ import BlasterBenchmarks.UPLC.Builtins
 import BlasterBenchmarks.UPLC.CekValue
 import BlasterBenchmarks.UPLC.Examples.Utils
 import BlasterBenchmarks.UPLC.Examples.Onchain.ProcessSCOrder.ProcessSCOrder
-import BlasterBenchmarks.UPLC.PreProcess
 import BlasterBenchmarks.UPLC.Uplc
 import Solver.Command.Tactic
 
@@ -15,109 +14,755 @@ set_option warn.sorry false
 -- STO3: Non-Negative N_RC
 -- STO4: Djed Reserve Backing Stablecoins
 -- STO5: Djed Reserve Backing Reservecoins
+
+-- Provable once subgoal splitting supported inherently in blaster
 theorem sto1_to_5 :
   ∀ (x : ProcessSCInput) (s : ComputeReserve),
   validOrderInput x →
-  resultToComputeReserve (fromHaltState $ prop_compiledProcessSCOrder x) = some s →
-  validReserve s := by sorry
-  -- intro x s
-  -- blaster (only-optimize: 1)
-  -- by_cases x.nbTokens > 0
-  -- . blaster
-  -- . by_cases x.state.crN_SC = 0 <;>
-  --   by_cases x.state.crN_RC = 0
-  --   . blaster
-  --   . blaster
-  --   . by_cases x.orderRate < mkRatio x.state.crReserve x.state.crN_SC
-  --     . let totalPrice := -(truncate $ x.orderRate * x.scBaseFeeSSC * fromInteger x.nbTokens)
-  --       let opFees := truncate $ fromInteger totalPrice * x.scOperatorFeeRatio
-  --       by_cases fromInteger opFees < fromInteger totalPrice * x.scOperatorFeeRatio
-  --       . by_cases 1 + opFees < x.scMinOperatorFee <;>
-  --         by_cases 1 + opFees < x.scMaxOperatorFee
-  --         . blaster
-  --         . blaster
-  --         . by_cases opFees < x.adaAtOrderUtxo - x.minAdaTransfer
-  --           . blaster
-  --           . by_cases x.orderRate * x.scBaseFeeSSC * x.scOperatorFeeRatio < zeroRatio <;> blaster (random-seed: 3)
-  --         . by_cases x.orderRate * x.scBaseFeeSSC * x.scOperatorFeeRatio < zeroRatio
-  --           . blaster
-  --           . by_cases x.adaAtOrderUtxo - x.minAdaTransfer < x.scMaxOperatorFee
-  --             . by_cases zeroRatio < x.orderRate * x.scBaseFeeSSC <;> blaster (random-seed: 14)
-  --             . blaster
-  --       . by_cases opFees < x.scMinOperatorFee <;>
-  --         by_cases opFees < x.scMaxOperatorFee
-  --         . blaster
-  --         . blaster
-  --         . by_cases x.adaAtOrderUtxo - x.minAdaTransfer < opFees
-  --           . by_cases x.orderRate * x.scBaseFeeSSC * x.scOperatorFeeRatio < zeroRatio <;> blaster (random-seed: 12)
-  --           . blaster
-  --         . by_cases x.orderRate * x.scBaseFeeSSC * x.scOperatorFeeRatio < zeroRatio
-  --           . blaster
-  --           . by_cases x.adaAtOrderUtxo - x.minAdaTransfer < x.scMaxOperatorFee
-  --             . by_cases zeroRatio < x.orderRate * x.scBaseFeeSSC <;> blaster (random-seed: 5)
-  --             . blaster
-  --     . let r_price := mkRatio x.state.crReserve x.state.crN_SC
-  --       let totalPrice := -(truncate $ r_price * x.scBaseFeeSSC * fromInteger x.nbTokens)
-  --       let opFees := truncate $ fromInteger totalPrice * x.scOperatorFeeRatio
-  --       by_cases fromInteger opFees < fromInteger totalPrice * x.scOperatorFeeRatio
-  --       . by_cases 1 + opFees < x.scMinOperatorFee <;>
-  --         by_cases 1 + opFees < x.scMaxOperatorFee
-  --         . blaster
-  --         . blaster
-  --         . by_cases opFees < x.adaAtOrderUtxo - x.minAdaTransfer
-  --           . blaster
-  --           . by_cases r_price * x.scBaseFeeSSC * x.scOperatorFeeRatio < zeroRatio <;> blaster
-  --         . by_cases r_price * x.scBaseFeeSSC * x.scOperatorFeeRatio < zeroRatio <;> blaster
-  --       . by_cases opFees < x.scMinOperatorFee <;>
-  --         by_cases opFees < x.scMaxOperatorFee
-  --         . blaster
-  --         . blaster
-  --         . by_cases opFees < x.adaAtOrderUtxo - x.minAdaTransfer
-  --           . blaster
-  --           . by_cases r_price * x.scBaseFeeSSC * x.scOperatorFeeRatio < zeroRatio <;> blaster (random-seed: 1)
-  --         . by_cases r_price * x.scBaseFeeSSC * x.scOperatorFeeRatio < zeroRatio <;> blaster (random-seed: 1)
-  --   . by_cases x.orderRate < fromInteger x.state.crReserve * (unsafeRecip $ fromInteger x.state.crN_SC * x.scBaseFeeBSC)
-  --     . let totalPrice := -(truncate $ x.orderRate * x.scBaseFeeSSC * fromInteger x.nbTokens)
-  --       let opFees := truncate $ fromInteger totalPrice * x.scOperatorFeeRatio
-  --       by_cases fromInteger opFees < fromInteger totalPrice * x.scOperatorFeeRatio
-  --       . by_cases 1 + opFees < x.scMinOperatorFee <;>
-  --         by_cases 1 + opFees < x.scMaxOperatorFee
-  --         . blaster
-  --         . blaster
-  --         . by_cases opFees < x.adaAtOrderUtxo - x.minAdaTransfer
-  --           . blaster
-  --           . by_cases x.orderRate * x.scBaseFeeSSC * x.scOperatorFeeRatio < zeroRatio <;> blaster (random-seed: 6)
-  --         . by_cases x.orderRate * x.scBaseFeeSSC * x.scOperatorFeeRatio < zeroRatio
-  --           . blaster
-  --           . by_cases x.adaAtOrderUtxo - x.minAdaTransfer < x.scMaxOperatorFee <;> blaster (random-seed: 5)
-  --       . by_cases opFees < x.scMinOperatorFee <;>
-  --         by_cases opFees < x.scMaxOperatorFee <;>
-  --         by_cases x.adaAtOrderUtxo - x.minAdaTransfer < opFees <;>
-  --         by_cases x.orderRate * x.scBaseFeeSSC * x.scOperatorFeeRatio < zeroRatio <;> blaster (random-seed: 4)
-  --     . let r_price := fromInteger x.state.crReserve * (unsafeRecip $ fromInteger x.state.crN_SC * x.scBaseFeeBSC)
-  --       let totalPrice := -(truncate $ r_price * x.scBaseFeeSSC * fromInteger x.nbTokens)
-  --       let opFees := truncate $ fromInteger totalPrice * x.scOperatorFeeRatio
-  --       by_cases fromInteger opFees < fromInteger totalPrice * x.scOperatorFeeRatio
-  --       . by_cases 1 + opFees < x.scMinOperatorFee <;>
-  --         by_cases 1 + opFees < x.scMaxOperatorFee
-  --         . blaster
-  --         . blaster
-  --         . by_cases opFees < x.adaAtOrderUtxo - x.minAdaTransfer <;>
-  --           by_cases r_price * x.scBaseFeeSSC * x.scOperatorFeeRatio < zeroRatio <;> blaster
-  --         . by_cases opFees < x.adaAtOrderUtxo - x.minAdaTransfer <;>
-  --           by_cases r_price * x.scBaseFeeSSC * x.scOperatorFeeRatio < zeroRatio <;> blaster (random-seed: 2)
-  --       . by_cases opFees < x.scMinOperatorFee <;>
-  --         by_cases opFees < x.scMaxOperatorFee
-  --         . blaster
-  --         . blaster
-  --         . by_cases x.adaAtOrderUtxo - x.minAdaTransfer < opFees <;>
-  --           by_cases r_price * x.scBaseFeeSSC * x.scOperatorFeeRatio < zeroRatio <;> blaster (random-seed: 9)
-  --         . by_cases x.adaAtOrderUtxo - x.minAdaTransfer < opFees <;>
-  --           by_cases r_price * x.scBaseFeeSSC * x.scOperatorFeeRatio < zeroRatio <;> blaster (random-seed: 7)
+  resultToComputeReserve (fromHaltState $ appliedProcessSCOrder x) = some s →
+  validReserve s :=
+  by sorry
 
 
--- NOTE: Remove solver options once subgoal splitting is supported
-#solve (timeout: 2) (solve-result: 2) [ sto1_to_5 ]
+-- Example of subgoal splitting to reduce complexity at Smt solver level
+theorem sto1_to_5_part1 :
+  ∀ (x : ProcessSCInput) (s : ComputeReserve),
+  x.nbTokens > 0 →
+  validOrderInput x →
+  resultToComputeReserve (fromHaltState $ appliedProcessSCOrder x) = some s →
+  validReserve s :=
+  by sorry
+
+theorem sto1_to_5_part2 :
+  ∀ (x : ProcessSCInput) (s : ComputeReserve),
+  x.nbTokens ≤ 0 →
+  x.state.crN_SC = 0 →
+  validOrderInput x →
+  resultToComputeReserve (fromHaltState $ appliedProcessSCOrder x) = some s →
+  validReserve s :=
+  by sorry
+
+theorem sto1_to_5_part3 :
+  ∀ (x : ProcessSCInput) (s : ComputeReserve),
+    let totalPrice := -(truncate $ x.orderRate * x.scBaseFeeSSC * fromInteger x.nbTokens)
+    let opFees := truncate $ fromInteger totalPrice * x.scOperatorFeeRatio
+    x.nbTokens ≤ 0 →
+    x.state.crN_SC ≠ 0 →
+    x.state.crN_RC = 0 →
+    x.orderRate < mkRatio x.state.crReserve x.state.crN_SC →
+    fromInteger opFees < fromInteger totalPrice * x.scOperatorFeeRatio →
+    1 + opFees < x.scMinOperatorFee →
+    validOrderInput x →
+    resultToComputeReserve (fromHaltState $ appliedProcessSCOrder x) = some s →
+    validReserve s :=
+    by sorry
+
+theorem sto1_to_5_part4 :
+  ∀ (x : ProcessSCInput) (s : ComputeReserve),
+    let totalPrice := -(truncate $ x.orderRate * x.scBaseFeeSSC * fromInteger x.nbTokens)
+    let opFees := truncate $ fromInteger totalPrice * x.scOperatorFeeRatio
+    x.nbTokens ≤ 0 →
+    x.state.crN_SC ≠ 0 →
+    x.state.crN_RC = 0 →
+    x.orderRate < mkRatio x.state.crReserve x.state.crN_SC →
+    fromInteger opFees < fromInteger totalPrice * x.scOperatorFeeRatio →
+    1 + opFees ≥ x.scMinOperatorFee →
+    1 + opFees < x.scMaxOperatorFee →
+    opFees < x.adaAtOrderUtxo - x.minAdaTransfer →
+    validOrderInput x →
+    resultToComputeReserve (fromHaltState $ appliedProcessSCOrder x) = some s →
+    validReserve s :=
+    by sorry
+
+theorem sto1_to_5_part5 :
+  ∀ (x : ProcessSCInput) (s : ComputeReserve),
+    let totalPrice := -(truncate $ x.orderRate * x.scBaseFeeSSC * fromInteger x.nbTokens)
+    let opFees := truncate $ fromInteger totalPrice * x.scOperatorFeeRatio
+    x.nbTokens ≤ 0 →
+    x.state.crN_SC ≠ 0 →
+    x.state.crN_RC = 0 →
+    x.orderRate < mkRatio x.state.crReserve x.state.crN_SC →
+    fromInteger opFees < fromInteger totalPrice * x.scOperatorFeeRatio →
+    1 + opFees ≥ x.scMinOperatorFee →
+    1 + opFees < x.scMaxOperatorFee →
+    opFees ≥ x.adaAtOrderUtxo - x.minAdaTransfer →
+    x.orderRate * x.scBaseFeeSSC * x.scOperatorFeeRatio < zeroRatio →
+    validOrderInput x →
+    resultToComputeReserve (fromHaltState $ appliedProcessSCOrder x) = some s →
+    validReserve s :=
+    by sorry
+
+theorem sto1_to_5_part6 :
+  ∀ (x : ProcessSCInput) (s : ComputeReserve),
+    let totalPrice := -(truncate $ x.orderRate * x.scBaseFeeSSC * fromInteger x.nbTokens)
+    let opFees := truncate $ fromInteger totalPrice * x.scOperatorFeeRatio
+    x.nbTokens ≤ 0 →
+    x.state.crN_SC ≠ 0 →
+    x.state.crN_RC = 0 →
+    x.orderRate < mkRatio x.state.crReserve x.state.crN_SC →
+    validOrderInput x →
+    fromInteger opFees < fromInteger totalPrice * x.scOperatorFeeRatio →
+    1 + opFees ≥ x.scMinOperatorFee →
+    1 + opFees < x.scMaxOperatorFee →
+    opFees ≥ x.adaAtOrderUtxo - x.minAdaTransfer →
+    x.orderRate * x.scBaseFeeSSC * x.scOperatorFeeRatio ≥ zeroRatio →
+    resultToComputeReserve (fromHaltState $ appliedProcessSCOrder x) = some s →
+    validReserve s :=
+    by sorry
+
+theorem sto1_to_5_part7 :
+  ∀ (x : ProcessSCInput) (s : ComputeReserve),
+    let totalPrice := -(truncate $ x.orderRate * x.scBaseFeeSSC * fromInteger x.nbTokens)
+    let opFees := truncate $ fromInteger totalPrice * x.scOperatorFeeRatio
+    x.nbTokens ≤ 0 →
+    x.state.crN_SC ≠ 0 →
+    x.state.crN_RC = 0 →
+    x.orderRate < mkRatio x.state.crReserve x.state.crN_SC →
+    validOrderInput x →
+    fromInteger opFees < fromInteger totalPrice * x.scOperatorFeeRatio →
+    1 + opFees ≥ x.scMinOperatorFee →
+    1 + opFees ≥ x.scMaxOperatorFee →
+    x.orderRate * x.scBaseFeeSSC * x.scOperatorFeeRatio < zeroRatio →
+    resultToComputeReserve (fromHaltState $ appliedProcessSCOrder x) = some s →
+    validReserve s :=
+    by sorry
+
+theorem sto1_to_5_part8 :
+  ∀ (x : ProcessSCInput) (s : ComputeReserve),
+    let totalPrice := -(truncate $ x.orderRate * x.scBaseFeeSSC * fromInteger x.nbTokens)
+    let opFees := truncate $ fromInteger totalPrice * x.scOperatorFeeRatio
+    x.nbTokens ≤ 0 →
+    x.state.crN_SC ≠ 0 →
+    x.state.crN_RC = 0 →
+    x.orderRate < mkRatio x.state.crReserve x.state.crN_SC →
+    validOrderInput x →
+    fromInteger opFees < fromInteger totalPrice * x.scOperatorFeeRatio →
+    1 + opFees ≥ x.scMinOperatorFee →
+    1 + opFees ≥ x.scMaxOperatorFee →
+    x.orderRate * x.scBaseFeeSSC * x.scOperatorFeeRatio ≥ zeroRatio →
+    zeroRatio ≥ x.orderRate * x.scBaseFeeSSC →
+    resultToComputeReserve (fromHaltState $ appliedProcessSCOrder x) = some s →
+    validReserve s :=
+    by sorry
+
+theorem sto1_to_5_part10 :
+  ∀ (x : ProcessSCInput) (s : ComputeReserve),
+    let totalPrice := -(truncate $ x.orderRate * x.scBaseFeeSSC * fromInteger x.nbTokens)
+    let opFees := truncate $ fromInteger totalPrice * x.scOperatorFeeRatio
+    x.nbTokens ≤ 0 →
+    x.state.crN_SC ≠ 0 →
+    x.state.crN_RC = 0 →
+    x.orderRate < mkRatio x.state.crReserve x.state.crN_SC →
+    validOrderInput x →
+    fromInteger opFees ≥ fromInteger totalPrice * x.scOperatorFeeRatio →
+    opFees < x.scMinOperatorFee →
+    resultToComputeReserve (fromHaltState $ appliedProcessSCOrder x) = some s →
+    validReserve s :=
+    by sorry
+
+theorem sto1_to_5_part11 :
+  ∀ (x : ProcessSCInput) (s : ComputeReserve),
+    let totalPrice := -(truncate $ x.orderRate * x.scBaseFeeSSC * fromInteger x.nbTokens)
+    let opFees := truncate $ fromInteger totalPrice * x.scOperatorFeeRatio
+    x.nbTokens ≤ 0 →
+    x.state.crN_SC ≠ 0 →
+    x.state.crN_RC = 0 →
+    x.orderRate < mkRatio x.state.crReserve x.state.crN_SC →
+    validOrderInput x →
+    fromInteger opFees ≥ fromInteger totalPrice * x.scOperatorFeeRatio →
+    opFees ≥ x.scMinOperatorFee →
+    opFees < x.scMaxOperatorFee →
+    x.adaAtOrderUtxo - x.minAdaTransfer < opFees →
+    x.orderRate * x.scBaseFeeSSC * x.scOperatorFeeRatio < zeroRatio →
+    resultToComputeReserve (fromHaltState $ appliedProcessSCOrder x) = some s →
+    validReserve s :=
+    by sorry
+
+theorem sto1_to_5_part12 :
+  ∀ (x : ProcessSCInput) (s : ComputeReserve),
+    let totalPrice := -(truncate $ x.orderRate * x.scBaseFeeSSC * fromInteger x.nbTokens)
+    let opFees := truncate $ fromInteger totalPrice * x.scOperatorFeeRatio
+    x.nbTokens ≤ 0 →
+    x.state.crN_SC ≠ 0 →
+    x.state.crN_RC = 0 →
+    x.orderRate < mkRatio x.state.crReserve x.state.crN_SC →
+    fromInteger opFees ≥ fromInteger totalPrice * x.scOperatorFeeRatio →
+    opFees ≥ x.scMinOperatorFee →
+    opFees < x.scMaxOperatorFee →
+    validOrderInput x →
+    x.adaAtOrderUtxo - x.minAdaTransfer ≥ opFees →
+    resultToComputeReserve (fromHaltState $ appliedProcessSCOrder x) = some s →
+    validReserve s :=
+    by sorry
+
+theorem sto1_to_5_part13 :
+  ∀ (x : ProcessSCInput) (s : ComputeReserve),
+    let totalPrice := -(truncate $ x.orderRate * x.scBaseFeeSSC * fromInteger x.nbTokens)
+    let opFees := truncate $ fromInteger totalPrice * x.scOperatorFeeRatio
+    x.nbTokens ≤ 0 →
+    x.state.crN_SC ≠ 0 →
+    x.state.crN_RC = 0 →
+    x.orderRate < mkRatio x.state.crReserve x.state.crN_SC →
+    fromInteger opFees ≥ fromInteger totalPrice * x.scOperatorFeeRatio →
+    opFees ≥ x.scMinOperatorFee →
+    opFees ≥ x.scMaxOperatorFee →
+    x.orderRate * x.scBaseFeeSSC * x.scOperatorFeeRatio < zeroRatio →
+    validOrderInput x →
+    resultToComputeReserve (fromHaltState $ appliedProcessSCOrder x) = some s →
+    validReserve s :=
+    by sorry
+
+theorem sto1_to_5_part14 :
+  ∀ (x : ProcessSCInput) (s : ComputeReserve),
+    let totalPrice := -(truncate $ x.orderRate * x.scBaseFeeSSC * fromInteger x.nbTokens)
+    let opFees := truncate $ fromInteger totalPrice * x.scOperatorFeeRatio
+    x.nbTokens ≤ 0 →
+    x.state.crN_SC ≠ 0 →
+    x.state.crN_RC = 0 →
+    x.orderRate < mkRatio x.state.crReserve x.state.crN_SC →
+    fromInteger opFees ≥ fromInteger totalPrice * x.scOperatorFeeRatio →
+    opFees ≥ x.scMinOperatorFee →
+    opFees ≥ x.scMaxOperatorFee →
+    x.orderRate * x.scBaseFeeSSC * x.scOperatorFeeRatio ≥ zeroRatio →
+    x.adaAtOrderUtxo - x.minAdaTransfer ≥ x.scMaxOperatorFee →
+    validOrderInput x →
+    resultToComputeReserve (fromHaltState $ appliedProcessSCOrder x) = some s →
+    validReserve s :=
+    by sorry
+
+
+theorem sto1_to_5_part15 :
+  ∀ (x : ProcessSCInput) (s : ComputeReserve),
+    let r_price := mkRatio x.state.crReserve x.state.crN_SC
+    let totalPrice := -(truncate $ r_price * x.scBaseFeeSSC * fromInteger x.nbTokens)
+    let opFees := truncate $ fromInteger totalPrice * x.scOperatorFeeRatio
+    x.nbTokens ≤ 0 →
+    x.state.crN_SC ≠ 0 →
+    x.state.crN_RC = 0 →
+    x.orderRate ≥ mkRatio x.state.crReserve x.state.crN_SC →
+    fromInteger opFees < fromInteger totalPrice * x.scOperatorFeeRatio →
+    1 + opFees < x.scMinOperatorFee →
+    validOrderInput x →
+    resultToComputeReserve (fromHaltState $ appliedProcessSCOrder x) = some s →
+    validReserve s :=
+    by sorry
+
+
+theorem sto1_to_5_part16 :
+  ∀ (x : ProcessSCInput) (s : ComputeReserve),
+    let r_price := mkRatio x.state.crReserve x.state.crN_SC
+    let totalPrice := -(truncate $ r_price * x.scBaseFeeSSC * fromInteger x.nbTokens)
+    let opFees := truncate $ fromInteger totalPrice * x.scOperatorFeeRatio
+    x.nbTokens ≤ 0 →
+    x.state.crN_SC ≠ 0 →
+    x.state.crN_RC = 0 →
+    x.orderRate ≥ mkRatio x.state.crReserve x.state.crN_SC →
+    fromInteger opFees < fromInteger totalPrice * x.scOperatorFeeRatio →
+    1 + opFees ≥ x.scMinOperatorFee →
+    1 + opFees < x.scMaxOperatorFee →
+    opFees < x.adaAtOrderUtxo - x.minAdaTransfer →
+    validOrderInput x →
+    resultToComputeReserve (fromHaltState $ appliedProcessSCOrder x) = some s →
+    validReserve s :=
+    by sorry
+
+theorem sto1_to_5_part17 :
+  ∀ (x : ProcessSCInput) (s : ComputeReserve),
+    let r_price := mkRatio x.state.crReserve x.state.crN_SC
+    let totalPrice := -(truncate $ r_price * x.scBaseFeeSSC * fromInteger x.nbTokens)
+    let opFees := truncate $ fromInteger totalPrice * x.scOperatorFeeRatio
+    x.nbTokens ≤ 0 →
+    x.state.crN_SC ≠ 0 →
+    x.state.crN_RC = 0 →
+    x.orderRate ≥ mkRatio x.state.crReserve x.state.crN_SC →
+    fromInteger opFees < fromInteger totalPrice * x.scOperatorFeeRatio →
+    1 + opFees ≥ x.scMinOperatorFee →
+    1 + opFees < x.scMaxOperatorFee →
+    opFees ≥ x.adaAtOrderUtxo - x.minAdaTransfer →
+    r_price * x.scBaseFeeSSC * x.scOperatorFeeRatio < zeroRatio →
+    validOrderInput x →
+    resultToComputeReserve (fromHaltState $ appliedProcessSCOrder x) = some s →
+    validReserve s :=
+    by sorry
+
+
+theorem sto1_to_5_part18 :
+  ∀ (x : ProcessSCInput) (s : ComputeReserve),
+    let r_price := mkRatio x.state.crReserve x.state.crN_SC
+    let totalPrice := -(truncate $ r_price * x.scBaseFeeSSC * fromInteger x.nbTokens)
+    let opFees := truncate $ fromInteger totalPrice * x.scOperatorFeeRatio
+    x.nbTokens ≤ 0 →
+    x.state.crN_SC ≠ 0 →
+    x.state.crN_RC = 0 →
+    x.orderRate ≥ mkRatio x.state.crReserve x.state.crN_SC →
+    fromInteger opFees < fromInteger totalPrice * x.scOperatorFeeRatio →
+    1 + opFees ≥ x.scMinOperatorFee →
+    1 + opFees < x.scMaxOperatorFee →
+    opFees ≥ x.adaAtOrderUtxo - x.minAdaTransfer →
+    r_price * x.scBaseFeeSSC * x.scOperatorFeeRatio ≥ zeroRatio →
+    validOrderInput x →
+    resultToComputeReserve (fromHaltState $ appliedProcessSCOrder x) = some s →
+    validReserve s :=
+    by sorry
+
+theorem sto1_to_5_part19 :
+  ∀ (x : ProcessSCInput) (s : ComputeReserve),
+    let r_price := mkRatio x.state.crReserve x.state.crN_SC
+    let totalPrice := -(truncate $ r_price * x.scBaseFeeSSC * fromInteger x.nbTokens)
+    let opFees := truncate $ fromInteger totalPrice * x.scOperatorFeeRatio
+    x.nbTokens ≤ 0 →
+    x.state.crN_SC ≠ 0 →
+    x.state.crN_RC = 0 →
+    x.orderRate ≥ mkRatio x.state.crReserve x.state.crN_SC →
+    validOrderInput x →
+    fromInteger opFees < fromInteger totalPrice * x.scOperatorFeeRatio →
+    1 + opFees ≥ x.scMinOperatorFee →
+    1 + opFees ≥ x.scMaxOperatorFee →
+    r_price * x.scBaseFeeSSC * x.scOperatorFeeRatio < zeroRatio →
+    resultToComputeReserve (fromHaltState $ appliedProcessSCOrder x) = some s →
+    validReserve s :=
+    by sorry
+
+theorem sto1_to_5_part20 :
+  ∀ (x : ProcessSCInput) (s : ComputeReserve),
+    let r_price := mkRatio x.state.crReserve x.state.crN_SC
+    let totalPrice := -(truncate $ r_price * x.scBaseFeeSSC * fromInteger x.nbTokens)
+    let opFees := truncate $ fromInteger totalPrice * x.scOperatorFeeRatio
+    x.nbTokens ≤ 0 →
+    x.state.crN_SC ≠ 0 →
+    x.state.crN_RC = 0 →
+    x.orderRate ≥ mkRatio x.state.crReserve x.state.crN_SC →
+    validOrderInput x →
+    fromInteger opFees < fromInteger totalPrice * x.scOperatorFeeRatio →
+    1 + opFees ≥ x.scMinOperatorFee →
+    1 + opFees ≥ x.scMaxOperatorFee →
+    r_price * x.scBaseFeeSSC * x.scOperatorFeeRatio ≥ zeroRatio →
+    resultToComputeReserve (fromHaltState $ appliedProcessSCOrder x) = some s →
+    validReserve s :=
+    by sorry
+
+theorem sto1_to_5_part21 :
+  ∀ (x : ProcessSCInput) (s : ComputeReserve),
+    let r_price := mkRatio x.state.crReserve x.state.crN_SC
+    let totalPrice := -(truncate $ r_price * x.scBaseFeeSSC * fromInteger x.nbTokens)
+    let opFees := truncate $ fromInteger totalPrice * x.scOperatorFeeRatio
+    x.nbTokens ≤ 0 →
+    x.state.crN_SC ≠ 0 →
+    x.state.crN_RC = 0 →
+    x.orderRate ≥ mkRatio x.state.crReserve x.state.crN_SC →
+    validOrderInput x →
+    fromInteger opFees ≥ fromInteger totalPrice * x.scOperatorFeeRatio →
+    opFees < x.scMinOperatorFee →
+    resultToComputeReserve (fromHaltState $ appliedProcessSCOrder x) = some s →
+    validReserve s :=
+    by sorry
+
+theorem sto1_to_5_part22 :
+  ∀ (x : ProcessSCInput) (s : ComputeReserve),
+    let r_price := mkRatio x.state.crReserve x.state.crN_SC
+    let totalPrice := -(truncate $ r_price * x.scBaseFeeSSC * fromInteger x.nbTokens)
+    let opFees := truncate $ fromInteger totalPrice * x.scOperatorFeeRatio
+    x.nbTokens ≤ 0 →
+    x.state.crN_SC ≠ 0 →
+    x.state.crN_RC = 0 →
+    x.orderRate ≥ mkRatio x.state.crReserve x.state.crN_SC →
+    validOrderInput x →
+    fromInteger opFees ≥ fromInteger totalPrice * x.scOperatorFeeRatio →
+    opFees ≥ x.scMinOperatorFee →
+    opFees < x.scMaxOperatorFee →
+    opFees < x.adaAtOrderUtxo - x.minAdaTransfer →
+    resultToComputeReserve (fromHaltState $ appliedProcessSCOrder x) = some s →
+    validReserve s :=
+    by sorry
+
+theorem sto1_to_5_part23 :
+  ∀ (x : ProcessSCInput) (s : ComputeReserve),
+    let r_price := mkRatio x.state.crReserve x.state.crN_SC
+    let totalPrice := -(truncate $ r_price * x.scBaseFeeSSC * fromInteger x.nbTokens)
+    let opFees := truncate $ fromInteger totalPrice * x.scOperatorFeeRatio
+    x.nbTokens ≤ 0 →
+    x.state.crN_SC ≠ 0 →
+    x.state.crN_RC = 0 →
+    x.orderRate ≥ mkRatio x.state.crReserve x.state.crN_SC →
+    validOrderInput x →
+    fromInteger opFees ≥ fromInteger totalPrice * x.scOperatorFeeRatio →
+    opFees ≥ x.scMinOperatorFee →
+    opFees < x.scMaxOperatorFee →
+    opFees ≥ x.adaAtOrderUtxo - x.minAdaTransfer →
+    r_price * x.scBaseFeeSSC * x.scOperatorFeeRatio < zeroRatio →
+    resultToComputeReserve (fromHaltState $ appliedProcessSCOrder x) = some s →
+    validReserve s :=
+    by sorry
+
+theorem sto1_to_5_part24 :
+  ∀ (x : ProcessSCInput) (s : ComputeReserve),
+    let r_price := mkRatio x.state.crReserve x.state.crN_SC
+    let totalPrice := -(truncate $ r_price * x.scBaseFeeSSC * fromInteger x.nbTokens)
+    let opFees := truncate $ fromInteger totalPrice * x.scOperatorFeeRatio
+    x.nbTokens ≤ 0 →
+    x.state.crN_SC ≠ 0 →
+    x.state.crN_RC = 0 →
+    x.orderRate ≥ mkRatio x.state.crReserve x.state.crN_SC →
+    validOrderInput x →
+    fromInteger opFees ≥ fromInteger totalPrice * x.scOperatorFeeRatio →
+    opFees ≥ x.scMinOperatorFee →
+    opFees < x.scMaxOperatorFee →
+    opFees ≥ x.adaAtOrderUtxo - x.minAdaTransfer →
+    r_price * x.scBaseFeeSSC * x.scOperatorFeeRatio ≥ zeroRatio →
+    resultToComputeReserve (fromHaltState $ appliedProcessSCOrder x) = some s →
+    validReserve s :=
+    by sorry
+
+theorem sto1_to_5_part25 :
+  ∀ (x : ProcessSCInput) (s : ComputeReserve),
+    let r_price := mkRatio x.state.crReserve x.state.crN_SC
+    let totalPrice := -(truncate $ r_price * x.scBaseFeeSSC * fromInteger x.nbTokens)
+    let opFees := truncate $ fromInteger totalPrice * x.scOperatorFeeRatio
+    x.nbTokens ≤ 0 →
+    x.state.crN_SC ≠ 0 →
+    x.state.crN_RC = 0 →
+    x.orderRate ≥ mkRatio x.state.crReserve x.state.crN_SC →
+    validOrderInput x →
+    fromInteger opFees ≥ fromInteger totalPrice * x.scOperatorFeeRatio →
+    opFees ≥ x.scMinOperatorFee →
+    opFees ≥ x.scMaxOperatorFee →
+    r_price * x.scBaseFeeSSC * x.scOperatorFeeRatio < zeroRatio →
+    resultToComputeReserve (fromHaltState $ appliedProcessSCOrder x) = some s →
+    validReserve s :=
+    by sorry
+
+theorem sto1_to_5_part26 :
+  ∀ (x : ProcessSCInput) (s : ComputeReserve),
+    let r_price := mkRatio x.state.crReserve x.state.crN_SC
+    let totalPrice := -(truncate $ r_price * x.scBaseFeeSSC * fromInteger x.nbTokens)
+    let opFees := truncate $ fromInteger totalPrice * x.scOperatorFeeRatio
+    x.nbTokens ≤ 0 →
+    x.state.crN_SC ≠ 0 →
+    x.state.crN_RC = 0 →
+    x.orderRate ≥ mkRatio x.state.crReserve x.state.crN_SC →
+    validOrderInput x →
+    fromInteger opFees ≥ fromInteger totalPrice * x.scOperatorFeeRatio →
+    opFees ≥ x.scMinOperatorFee →
+    opFees ≥ x.scMaxOperatorFee →
+    r_price * x.scBaseFeeSSC * x.scOperatorFeeRatio ≥ zeroRatio →
+    resultToComputeReserve (fromHaltState $ appliedProcessSCOrder x) = some s →
+    validReserve s :=
+    by sorry
+
+theorem sto1_to_5_part27 :
+  ∀ (x : ProcessSCInput) (s : ComputeReserve),
+    let totalPrice := -(truncate $ x.orderRate * x.scBaseFeeSSC * fromInteger x.nbTokens)
+    let opFees := truncate $ fromInteger totalPrice * x.scOperatorFeeRatio
+    x.nbTokens ≤ 0 →
+    x.state.crN_SC ≠ 0 →
+    x.state.crN_RC ≠ 0 →
+    x.orderRate < fromInteger x.state.crReserve * (unsafeRecip $ fromInteger x.state.crN_SC * x.scBaseFeeBSC) →
+    validOrderInput x →
+    fromInteger opFees < fromInteger totalPrice * x.scOperatorFeeRatio →
+    1 + opFees < x.scMinOperatorFee →
+    resultToComputeReserve (fromHaltState $ appliedProcessSCOrder x) = some s →
+    validReserve s :=
+    by sorry
+
+theorem sto1_to_5_part28 :
+  ∀ (x : ProcessSCInput) (s : ComputeReserve),
+    let totalPrice := -(truncate $ x.orderRate * x.scBaseFeeSSC * fromInteger x.nbTokens)
+    let opFees := truncate $ fromInteger totalPrice * x.scOperatorFeeRatio
+    x.nbTokens ≤ 0 →
+    x.state.crN_SC ≠ 0 →
+    x.state.crN_RC ≠ 0 →
+    x.orderRate < fromInteger x.state.crReserve * (unsafeRecip $ fromInteger x.state.crN_SC * x.scBaseFeeBSC) →
+    validOrderInput x →
+    fromInteger opFees < fromInteger totalPrice * x.scOperatorFeeRatio →
+    1 + opFees ≥ x.scMinOperatorFee →
+    1 + opFees < x.scMaxOperatorFee →
+    opFees < x.adaAtOrderUtxo - x.minAdaTransfer →
+    resultToComputeReserve (fromHaltState $ appliedProcessSCOrder x) = some s →
+    validReserve s :=
+    by sorry
+
+theorem sto1_to_5_part29 :
+  ∀ (x : ProcessSCInput) (s : ComputeReserve),
+    let totalPrice := -(truncate $ x.orderRate * x.scBaseFeeSSC * fromInteger x.nbTokens)
+    let opFees := truncate $ fromInteger totalPrice * x.scOperatorFeeRatio
+    x.nbTokens ≤ 0 →
+    x.state.crN_SC ≠ 0 →
+    x.state.crN_RC ≠ 0 →
+    x.orderRate < fromInteger x.state.crReserve * (unsafeRecip $ fromInteger x.state.crN_SC * x.scBaseFeeBSC) →
+    fromInteger opFees < fromInteger totalPrice * x.scOperatorFeeRatio →
+    1 + opFees ≥ x.scMinOperatorFee →
+    1 + opFees < x.scMaxOperatorFee →
+    opFees ≥ x.adaAtOrderUtxo - x.minAdaTransfer →
+    x.orderRate * x.scBaseFeeSSC * x.scOperatorFeeRatio < zeroRatio →
+    validOrderInput x →
+    resultToComputeReserve (fromHaltState $ appliedProcessSCOrder x) = some s →
+    validReserve s :=
+    by sorry
+
+theorem sto1_to_5_part30 :
+  ∀ (x : ProcessSCInput) (s : ComputeReserve),
+    let totalPrice := -(truncate $ x.orderRate * x.scBaseFeeSSC * fromInteger x.nbTokens)
+    let opFees := truncate $ fromInteger totalPrice * x.scOperatorFeeRatio
+    x.nbTokens ≤ 0 →
+    x.state.crN_SC ≠ 0 →
+    x.state.crN_RC ≠ 0 →
+    x.orderRate < fromInteger x.state.crReserve * (unsafeRecip $ fromInteger x.state.crN_SC * x.scBaseFeeBSC) →
+    fromInteger opFees < fromInteger totalPrice * x.scOperatorFeeRatio →
+    validOrderInput x →
+    1 + opFees ≥ x.scMinOperatorFee →
+    1 + opFees < x.scMaxOperatorFee →
+    opFees ≥ x.adaAtOrderUtxo - x.minAdaTransfer →
+    x.orderRate * x.scBaseFeeSSC * x.scOperatorFeeRatio ≥ zeroRatio →
+    resultToComputeReserve (fromHaltState $ appliedProcessSCOrder x) = some s →
+    validReserve s :=
+    by sorry
+
+theorem sto1_to_5_part31 :
+  ∀ (x : ProcessSCInput) (s : ComputeReserve),
+    let totalPrice := -(truncate $ x.orderRate * x.scBaseFeeSSC * fromInteger x.nbTokens)
+    let opFees := truncate $ fromInteger totalPrice * x.scOperatorFeeRatio
+    x.nbTokens ≤ 0 →
+    x.state.crN_SC ≠ 0 →
+    x.state.crN_RC ≠ 0 →
+    x.orderRate < fromInteger x.state.crReserve * (unsafeRecip $ fromInteger x.state.crN_SC * x.scBaseFeeBSC) →
+    fromInteger opFees ≥ fromInteger totalPrice * x.scOperatorFeeRatio →
+    validOrderInput x →
+    opFees < x.scMinOperatorFee →
+    resultToComputeReserve (fromHaltState $ appliedProcessSCOrder x) = some s →
+    validReserve s :=
+    by sorry
+
+theorem sto1_to_5_part32 :
+  ∀ (x : ProcessSCInput) (s : ComputeReserve),
+    let totalPrice := -(truncate $ x.orderRate * x.scBaseFeeSSC * fromInteger x.nbTokens)
+    let opFees := truncate $ fromInteger totalPrice * x.scOperatorFeeRatio
+    x.nbTokens ≤ 0 →
+    x.state.crN_SC ≠ 0 →
+    x.state.crN_RC ≠ 0 →
+    x.orderRate < fromInteger x.state.crReserve * (unsafeRecip $ fromInteger x.state.crN_SC * x.scBaseFeeBSC) →
+    fromInteger opFees ≥ fromInteger totalPrice * x.scOperatorFeeRatio →
+    validOrderInput x →
+    opFees ≥ x.scMinOperatorFee →
+    opFees < x.scMaxOperatorFee →
+    x.orderRate * x.scBaseFeeSSC * x.scOperatorFeeRatio < zeroRatio →
+    resultToComputeReserve (fromHaltState $ appliedProcessSCOrder x) = some s →
+    validReserve s :=
+    by sorry
+
+theorem sto1_to_5_part33 :
+  ∀ (x : ProcessSCInput) (s : ComputeReserve),
+    let totalPrice := -(truncate $ x.orderRate * x.scBaseFeeSSC * fromInteger x.nbTokens)
+    let opFees := truncate $ fromInteger totalPrice * x.scOperatorFeeRatio
+    x.nbTokens ≤ 0 →
+    x.state.crN_SC ≠ 0 →
+    x.state.crN_RC ≠ 0 →
+    x.orderRate < fromInteger x.state.crReserve * (unsafeRecip $ fromInteger x.state.crN_SC * x.scBaseFeeBSC) →
+    fromInteger opFees ≥ fromInteger totalPrice * x.scOperatorFeeRatio →
+    validOrderInput x →
+    opFees ≥ x.scMinOperatorFee →
+    opFees < x.scMaxOperatorFee →
+    x.orderRate * x.scBaseFeeSSC * x.scOperatorFeeRatio ≥ zeroRatio →
+    x.adaAtOrderUtxo - x.minAdaTransfer ≥ opFees →
+    resultToComputeReserve (fromHaltState $ appliedProcessSCOrder x) = some s →
+    validReserve s :=
+    by sorry
+
+theorem sto1_to_5_part34 :
+  ∀ (x : ProcessSCInput) (s : ComputeReserve),
+    let totalPrice := -(truncate $ x.orderRate * x.scBaseFeeSSC * fromInteger x.nbTokens)
+    let opFees := truncate $ fromInteger totalPrice * x.scOperatorFeeRatio
+    x.nbTokens ≤ 0 →
+    x.state.crN_SC ≠ 0 →
+    x.state.crN_RC ≠ 0 →
+    x.orderRate < fromInteger x.state.crReserve * (unsafeRecip $ fromInteger x.state.crN_SC * x.scBaseFeeBSC) →
+    fromInteger opFees ≥ fromInteger totalPrice * x.scOperatorFeeRatio →
+    validOrderInput x →
+    opFees ≥ x.scMinOperatorFee →
+    opFees < x.scMaxOperatorFee →
+    x.orderRate * x.scBaseFeeSSC * x.scOperatorFeeRatio ≥ zeroRatio →
+    x.adaAtOrderUtxo - x.minAdaTransfer < opFees →
+    resultToComputeReserve (fromHaltState $ appliedProcessSCOrder x) = some s →
+    validReserve s :=
+    by sorry
+
+theorem sto1_to_5_part35 :
+  ∀ (x : ProcessSCInput) (s : ComputeReserve),
+    let totalPrice := -(truncate $ x.orderRate * x.scBaseFeeSSC * fromInteger x.nbTokens)
+    let opFees := truncate $ fromInteger totalPrice * x.scOperatorFeeRatio
+    x.nbTokens ≤ 0 →
+    x.state.crN_SC ≠ 0 →
+    x.state.crN_RC ≠ 0 →
+    x.orderRate < fromInteger x.state.crReserve * (unsafeRecip $ fromInteger x.state.crN_SC * x.scBaseFeeBSC) →
+    fromInteger opFees ≥ fromInteger totalPrice * x.scOperatorFeeRatio →
+    validOrderInput x →
+    opFees ≥ x.scMinOperatorFee →
+    opFees < x.scMaxOperatorFee →
+    x.orderRate * x.scBaseFeeSSC * x.scOperatorFeeRatio ≥ zeroRatio →
+    x.adaAtOrderUtxo - x.minAdaTransfer ≥ opFees →
+    resultToComputeReserve (fromHaltState $ appliedProcessSCOrder x) = some s →
+    validReserve s :=
+    by sorry
+
+theorem sto1_to_5_part36 :
+  ∀ (x : ProcessSCInput) (s : ComputeReserve),
+    let r_price := fromInteger x.state.crReserve * (unsafeRecip $ fromInteger x.state.crN_SC * x.scBaseFeeBSC)
+    let totalPrice := -(truncate $ r_price * x.scBaseFeeSSC * fromInteger x.nbTokens)
+    let opFees := truncate $ fromInteger totalPrice * x.scOperatorFeeRatio
+    x.nbTokens ≤ 0 →
+    x.state.crN_SC ≠ 0 →
+    x.state.crN_RC ≠ 0 →
+    x.orderRate ≥ fromInteger x.state.crReserve * (unsafeRecip $ fromInteger x.state.crN_SC * x.scBaseFeeBSC) →
+    fromInteger opFees < fromInteger totalPrice * x.scOperatorFeeRatio →
+    validOrderInput x →
+    1 + opFees < x.scMinOperatorFee →
+    resultToComputeReserve (fromHaltState $ appliedProcessSCOrder x) = some s →
+    validReserve s :=
+    by sorry
+
+theorem sto1_to_5_part37 :
+  ∀ (x : ProcessSCInput) (s : ComputeReserve),
+    let r_price := fromInteger x.state.crReserve * (unsafeRecip $ fromInteger x.state.crN_SC * x.scBaseFeeBSC)
+    let totalPrice := -(truncate $ r_price * x.scBaseFeeSSC * fromInteger x.nbTokens)
+    let opFees := truncate $ fromInteger totalPrice * x.scOperatorFeeRatio
+    x.nbTokens ≤ 0 →
+    x.state.crN_SC ≠ 0 →
+    x.state.crN_RC ≠ 0 →
+    x.orderRate ≥ fromInteger x.state.crReserve * (unsafeRecip $ fromInteger x.state.crN_SC * x.scBaseFeeBSC) →
+    fromInteger opFees < fromInteger totalPrice * x.scOperatorFeeRatio →
+    validOrderInput x →
+    1 + opFees ≥ x.scMinOperatorFee →
+    1 + opFees < x.scMaxOperatorFee →
+    opFees < x.adaAtOrderUtxo - x.minAdaTransfer →
+    resultToComputeReserve (fromHaltState $ appliedProcessSCOrder x) = some s →
+    validReserve s :=
+    by sorry
+
+theorem sto1_to_5_part38 :
+  ∀ (x : ProcessSCInput) (s : ComputeReserve),
+    let r_price := fromInteger x.state.crReserve * (unsafeRecip $ fromInteger x.state.crN_SC * x.scBaseFeeBSC)
+    let totalPrice := -(truncate $ r_price * x.scBaseFeeSSC * fromInteger x.nbTokens)
+    let opFees := truncate $ fromInteger totalPrice * x.scOperatorFeeRatio
+    x.nbTokens ≤ 0 →
+    x.state.crN_SC ≠ 0 →
+    x.state.crN_RC ≠ 0 →
+    x.orderRate ≥ fromInteger x.state.crReserve * (unsafeRecip $ fromInteger x.state.crN_SC * x.scBaseFeeBSC) →
+    fromInteger opFees < fromInteger totalPrice * x.scOperatorFeeRatio →
+    validOrderInput x →
+    1 + opFees ≥ x.scMinOperatorFee →
+    1 + opFees < x.scMaxOperatorFee →
+    opFees ≥ x.adaAtOrderUtxo - x.minAdaTransfer →
+    r_price * x.scBaseFeeSSC * x.scOperatorFeeRatio < zeroRatio →
+    resultToComputeReserve (fromHaltState $ appliedProcessSCOrder x) = some s →
+    validReserve s :=
+    by sorry
+
+
+theorem sto1_to_5_part39 :
+  ∀ (x : ProcessSCInput) (s : ComputeReserve),
+    let r_price := fromInteger x.state.crReserve * (unsafeRecip $ fromInteger x.state.crN_SC * x.scBaseFeeBSC)
+    let totalPrice := -(truncate $ r_price * x.scBaseFeeSSC * fromInteger x.nbTokens)
+    let opFees := truncate $ fromInteger totalPrice * x.scOperatorFeeRatio
+    x.nbTokens ≤ 0 →
+    x.state.crN_SC ≠ 0 →
+    x.state.crN_RC ≠ 0 →
+    x.orderRate ≥ fromInteger x.state.crReserve * (unsafeRecip $ fromInteger x.state.crN_SC * x.scBaseFeeBSC) →
+    fromInteger opFees < fromInteger totalPrice * x.scOperatorFeeRatio →
+    validOrderInput x →
+    1 + opFees ≥ x.scMinOperatorFee →
+    1 + opFees < x.scMaxOperatorFee →
+    opFees ≥ x.adaAtOrderUtxo - x.minAdaTransfer →
+    r_price * x.scBaseFeeSSC * x.scOperatorFeeRatio ≥ zeroRatio →
+    resultToComputeReserve (fromHaltState $ appliedProcessSCOrder x) = some s →
+    validReserve s :=
+    by sorry
+
+theorem sto1_to_5_part40 :
+  ∀ (x : ProcessSCInput) (s : ComputeReserve),
+    let r_price := fromInteger x.state.crReserve * (unsafeRecip $ fromInteger x.state.crN_SC * x.scBaseFeeBSC)
+    let totalPrice := -(truncate $ r_price * x.scBaseFeeSSC * fromInteger x.nbTokens)
+    let opFees := truncate $ fromInteger totalPrice * x.scOperatorFeeRatio
+    x.nbTokens ≤ 0 →
+    x.state.crN_SC ≠ 0 →
+    x.state.crN_RC ≠ 0 →
+    x.orderRate ≥ fromInteger x.state.crReserve * (unsafeRecip $ fromInteger x.state.crN_SC * x.scBaseFeeBSC) →
+    fromInteger opFees ≥ fromInteger totalPrice * x.scOperatorFeeRatio →
+    validOrderInput x →
+    opFees < x.scMinOperatorFee →
+    resultToComputeReserve (fromHaltState $ appliedProcessSCOrder x) = some s →
+    validReserve s :=
+    by sorry
+
+theorem sto1_to_5_part41 :
+  ∀ (x : ProcessSCInput) (s : ComputeReserve),
+    let r_price := fromInteger x.state.crReserve * (unsafeRecip $ fromInteger x.state.crN_SC * x.scBaseFeeBSC)
+    let totalPrice := -(truncate $ r_price * x.scBaseFeeSSC * fromInteger x.nbTokens)
+    let opFees := truncate $ fromInteger totalPrice * x.scOperatorFeeRatio
+    x.nbTokens ≤ 0 →
+    x.state.crN_SC ≠ 0 →
+    x.state.crN_RC ≠ 0 →
+    x.orderRate ≥ fromInteger x.state.crReserve * (unsafeRecip $ fromInteger x.state.crN_SC * x.scBaseFeeBSC) →
+    fromInteger opFees ≥ fromInteger totalPrice * x.scOperatorFeeRatio →
+    validOrderInput x →
+    opFees ≥ x.scMinOperatorFee →
+    opFees < x.scMaxOperatorFee →
+    r_price * x.scBaseFeeSSC * x.scOperatorFeeRatio < zeroRatio →
+    resultToComputeReserve (fromHaltState $ appliedProcessSCOrder x) = some s →
+    validReserve s :=
+    by sorry
+
+theorem sto1_to_5_part42 :
+  ∀ (x : ProcessSCInput) (s : ComputeReserve),
+    let r_price := fromInteger x.state.crReserve * (unsafeRecip $ fromInteger x.state.crN_SC * x.scBaseFeeBSC)
+    let totalPrice := -(truncate $ r_price * x.scBaseFeeSSC * fromInteger x.nbTokens)
+    let opFees := truncate $ fromInteger totalPrice * x.scOperatorFeeRatio
+    x.nbTokens ≤ 0 →
+    x.state.crN_SC ≠ 0 →
+    x.state.crN_RC ≠ 0 →
+    x.orderRate ≥ fromInteger x.state.crReserve * (unsafeRecip $ fromInteger x.state.crN_SC * x.scBaseFeeBSC) →
+    fromInteger opFees ≥ fromInteger totalPrice * x.scOperatorFeeRatio →
+    validOrderInput x →
+    opFees ≥ x.scMinOperatorFee →
+    opFees < x.scMaxOperatorFee →
+    r_price * x.scBaseFeeSSC * x.scOperatorFeeRatio ≥ zeroRatio →
+    resultToComputeReserve (fromHaltState $ appliedProcessSCOrder x) = some s →
+    validReserve s :=
+    by sorry
+
+theorem sto1_to_5_part43 :
+  ∀ (x : ProcessSCInput) (s : ComputeReserve),
+    let r_price := fromInteger x.state.crReserve * (unsafeRecip $ fromInteger x.state.crN_SC * x.scBaseFeeBSC)
+    let totalPrice := -(truncate $ r_price * x.scBaseFeeSSC * fromInteger x.nbTokens)
+    let opFees := truncate $ fromInteger totalPrice * x.scOperatorFeeRatio
+    x.nbTokens ≤ 0 →
+    x.state.crN_SC ≠ 0 →
+    x.state.crN_RC ≠ 0 →
+    x.orderRate ≥ fromInteger x.state.crReserve * (unsafeRecip $ fromInteger x.state.crN_SC * x.scBaseFeeBSC) →
+    fromInteger opFees ≥ fromInteger totalPrice * x.scOperatorFeeRatio →
+    validOrderInput x →
+    opFees ≥ x.scMinOperatorFee →
+    opFees ≥ x.scMaxOperatorFee →
+    r_price * x.scBaseFeeSSC * x.scOperatorFeeRatio < zeroRatio →
+    resultToComputeReserve (fromHaltState $ appliedProcessSCOrder x) = some s →
+    validReserve s :=
+    by sorry
+
+theorem sto1_to_5_part44 :
+  ∀ (x : ProcessSCInput) (s : ComputeReserve),
+    let r_price := fromInteger x.state.crReserve * (unsafeRecip $ fromInteger x.state.crN_SC * x.scBaseFeeBSC)
+    let totalPrice := -(truncate $ r_price * x.scBaseFeeSSC * fromInteger x.nbTokens)
+    let opFees := truncate $ fromInteger totalPrice * x.scOperatorFeeRatio
+    x.nbTokens ≤ 0 →
+    x.state.crN_SC ≠ 0 →
+    x.state.crN_RC ≠ 0 →
+    x.orderRate ≥ fromInteger x.state.crReserve * (unsafeRecip $ fromInteger x.state.crN_SC * x.scBaseFeeBSC) →
+    fromInteger opFees ≥ fromInteger totalPrice * x.scOperatorFeeRatio →
+    validOrderInput x →
+    opFees ≥ x.scMinOperatorFee →
+    opFees ≥ x.scMaxOperatorFee →
+    r_price * x.scBaseFeeSSC * x.scOperatorFeeRatio < zeroRatio →
+    resultToComputeReserve (fromHaltState $ appliedProcessSCOrder x) = some s →
+    validReserve s :=
+    by sorry
 
 
 end Tests.Uplc.Onchain.ProcessSCOrder
