BlasterBenchmarks/UPLC/Examples/Onchain/ProcessSCOrder/STO35.lean
@@ -2,7 +2,6 @@ import BlasterBenchmarks.UPLC.Builtins
 import BlasterBenchmarks.UPLC.CekValue
 import BlasterBenchmarks.UPLC.Examples.Utils
 import BlasterBenchmarks.UPLC.Examples.Onchain.ProcessSCOrder.ProcessSCOrder
-import BlasterBenchmarks.UPLC.PreProcess
 import BlasterBenchmarks.UPLC.Uplc
 import Solver.Command.Tactic
 
@@ -16,12 +15,8 @@ theorem sto35 :
   ∀ (x : ProcessSCInput),
     isBuySCOrder x →
     validOrderInput x →
-    isMaxStablecoinMintingReachedStatus (fromHaltState $ prop_compiledProcessSCOrder x) →
+    isMaxStablecoinMintingReachedStatus (fromHaltState $ appliedProcessSCOrder x) →
     validMaxMintingViolation x := by sorry
-    -- blaster (only-optimize: 1)
-
--- Proved only with optimization rules
-#solve (only-optimize: 1) [ sto35 ]
 
 
 end Tests.Uplc.Onchain.ProcessSCOrder
