BlasterBenchmarks/UPLC/Examples/Onchain/ProcessSCOrder/STO45.lean
@@ -2,40 +2,85 @@ import BlasterBenchmarks.UPLC.Builtins
 import BlasterBenchmarks.UPLC.CekValue
 import BlasterBenchmarks.UPLC.Examples.Utils
 import BlasterBenchmarks.UPLC.Examples.Onchain.ProcessSCOrder.ProcessSCOrder
-import BlasterBenchmarks.UPLC.PreProcess
 import BlasterBenchmarks.UPLC.Uplc
 import Solver.Command.Tactic
 
 namespace Tests.Uplc.Onchain.ProcessSCOrder
 open Tests.Uplc.Onchain
 
--- STO45: Insufficient Operator’s Fees Violation for Selling Stablecoin Order
-
 set_option warn.sorry false
--- NOTE: Example of subgoal splitting to reduce complexity at Smt solver level
+-- STO45: Insufficient Operator’s Fees Violation for Selling Stablecoin Order
+-- Provable once subgoal splitting supported inherently in blaster
 theorem sto45 :
   ∀ (x : ProcessSCInput),
   isSellSCOrder x →
   validOrderInput x →
-  isInsufficientOperatorFees (fromHaltState $ prop_compiledProcessSCOrder x) →
+  isInsufficientOperatorFees (fromHaltState $ appliedProcessSCOrder x) →
   validInsufficientFeesForSellSC x := by sorry
-  -- intro x;
-  -- blaster (only-optimize: 1)
-  -- by_cases x.state.crN_SC = 0 <;>
-  -- by_cases x.state.crN_RC = 0
-  -- . blaster
-  -- . blaster
-  -- . by_cases x.orderRate < mkRatio x.state.crReserve x.state.crN_SC <;> blaster
-  -- . by_cases x.orderRate < fromInteger x.state.crReserve * (unsafeRecip $ fromInteger x.state.crN_SC * x.scBaseFeeBSC)
-  --   . blaster
-  --   . let price := fromInteger x.state.crReserve * (unsafeRecip $ fromInteger x.state.crN_SC * x.scBaseFeeBSC)
-  --     let priceWithFees := (price * x.scBaseFeeSSC) * x.scOperatorFeeRatio
-  --     by_cases fromInteger (truncate priceWithFees) < priceWithFees
-  --     . blaster (random-seed: 4)
-  --     . blaster
 
--- NOTE: Remove solver options once subgoal splitting is supported
-#solve (timeout: 2) (solve-result: 2) [ sto45 ]
+-- Example of subgoal splitting to reduce complexity at Smt solver level
+theorem sto45_part1 :
+  ∀ (x : ProcessSCInput),
+  isSellSCOrder x →
+  validOrderInput x →
+  x.state.crN_SC = 0 →
+  isInsufficientOperatorFees (fromHaltState $ appliedProcessSCOrder x) →
+  validInsufficientFeesForSellSC x := by sorry
 
+theorem sto45_part2 :
+  ∀ (x : ProcessSCInput),
+  isSellSCOrder x →
+  validOrderInput x →
+  x.state.crN_SC ≠ 0 →
+  x.state.crN_RC = 0 →
+  x.orderRate < mkRatio x.state.crReserve x.state.crN_SC →
+  isInsufficientOperatorFees (fromHaltState $ appliedProcessSCOrder x) →
+  validInsufficientFeesForSellSC x := by sorry
+
+theorem sto45_part3 :
+  ∀ (x : ProcessSCInput),
+  isSellSCOrder x →
+  validOrderInput x →
+  x.state.crN_SC ≠ 0 →
+  x.state.crN_RC = 0 →
+  x.orderRate ≥ mkRatio x.state.crReserve x.state.crN_SC →
+  isInsufficientOperatorFees (fromHaltState $ appliedProcessSCOrder x) →
+  validInsufficientFeesForSellSC x := by sorry
+
+theorem sto45_part4 :
+  ∀ (x : ProcessSCInput),
+  isSellSCOrder x →
+  validOrderInput x →
+  x.state.crN_SC ≠ 0 →
+  x.state.crN_RC ≠ 0 →
+  x.orderRate < fromInteger x.state.crReserve * (unsafeRecip $ fromInteger x.state.crN_SC * x.scBaseFeeBSC) →
+  isInsufficientOperatorFees (fromHaltState $ appliedProcessSCOrder x) →
+  validInsufficientFeesForSellSC x := by sorry
+
+theorem sto45_part5 :
+  ∀ (x : ProcessSCInput),
+  isSellSCOrder x →
+  validOrderInput x →
+  x.state.crN_SC ≠ 0 →
+  x.state.crN_RC ≠ 0 →
+  x.orderRate ≥ fromInteger x.state.crReserve * (unsafeRecip $ fromInteger x.state.crN_SC * x.scBaseFeeBSC) →
+  let price := fromInteger x.state.crReserve * (unsafeRecip $ fromInteger x.state.crN_SC * x.scBaseFeeBSC)
+  let priceWithFees := (price * x.scBaseFeeSSC) * x.scOperatorFeeRatio
+  fromInteger (truncate priceWithFees) < priceWithFees →
+  isInsufficientOperatorFees (fromHaltState $ appliedProcessSCOrder x) →
+  validInsufficientFeesForSellSC x := by sorry
+
+theorem sto45_part6 :
+  ∀ (x : ProcessSCInput),
+  let price := fromInteger x.state.crReserve * (unsafeRecip $ fromInteger x.state.crN_SC * x.scBaseFeeBSC)
+  let priceWithFees := (price * x.scBaseFeeSSC) * x.scOperatorFeeRatio
+  fromInteger (truncate priceWithFees) ≥ priceWithFees →
+  isSellSCOrder x →
+  validOrderInput x →
+  x.state.crN_SC ≠ 0 →
+  x.state.crN_RC ≠ 0 →
+  x.orderRate ≥ fromInteger x.state.crReserve * (unsafeRecip $ fromInteger x.state.crN_SC * x.scBaseFeeBSC) →
+  isInsufficientOperatorFees (fromHaltState $ appliedProcessSCOrder x) →
+  validInsufficientFeesForSellSC x := by sorry
 
 end Tests.Uplc.Onchain.ProcessSCOrder
