BlasterBenchmarks/UPLC/Examples/Onchain/ProcessSCOrder/STO7.lean
@@ -2,7 +2,6 @@ import BlasterBenchmarks.UPLC.Builtins
 import BlasterBenchmarks.UPLC.CekValue
 import BlasterBenchmarks.UPLC.Examples.Utils
 import BlasterBenchmarks.UPLC.Examples.Onchain.ProcessSCOrder.ProcessSCOrder
-import BlasterBenchmarks.UPLC.PreProcess
 import BlasterBenchmarks.UPLC.Uplc
 import Solver.Command.Tactic
 
@@ -10,27 +9,29 @@ namespace Tests.Uplc.Onchain.ProcessSCOrder
 open Tests.Uplc.Onchain
 
 set_option warn.sorry false
--- set_option pp.deepTerms.threshold 50000 in
--- set_option pp.deepTerms true in
--- set_option pp.maxSteps 50000 in
--- set_option trace.Translate.optExpr true in
-
 -- STO7: Successful Buying Stablecoin Order
+
+-- Provable once subgoal splitting supported inherently in blaster
 theorem sto7 :
-  ∀ (x : ProcessSCInput) (s : ComputeReserve),
+  ∀ (x : ProcessSCInput),
    isBuySCOrder x →
    validOrderInput x →
-   resultToComputeReserve (fromHaltState $ prop_compiledProcessSCOrder x) = some s →
-   validBuySC x s := by sorry
-  --  intro x s;
-  --  blaster (only-optimize: 1)
-  --  by_cases x.state.crN_RC = 0
-  --  . let price := fromInteger x.nbTokens * (x.orderRate * x.scBaseFeeBSC)
-  --    by_cases fromInteger (truncate price) < price <;> blaster
-  --  . blaster (random-seed: 3) (timeout: 5)
+   successfulOrderImpliesPredicate (fromHaltState $ appliedProcessSCOrder x) (validBuySC x) := by sorry
 
--- NOTE: Remove solver options once subgoal splitting is supported
-#solve (timeout: 10) (solve-result: 2) [ sto7 ]
+-- Example of subgoal splitting to reduce complexity at Smt solver level
+theorem sto7_part1 :
+  ∀ (x : ProcessSCInput),
+   isBuySCOrder x →
+   validOrderInput x →
+   x.state.crN_RC = 0 →
+   successfulOrderImpliesPredicate (fromHaltState $ appliedProcessSCOrder x) (validBuySC x) := by sorry
+
+theorem sto7_part2 :
+  ∀ (x : ProcessSCInput),
+   isBuySCOrder x →
+   validOrderInput x →
+   x.state.crN_RC ≠ 0 →
+   successfulOrderImpliesPredicate (fromHaltState $ appliedProcessSCOrder x) (validBuySC x) := by sorry
 
 
 end Tests.Uplc.Onchain.ProcessSCOrder
