BlasterBenchmarks/UPLC/Examples/Onchain/ProcessSCOrder/STO8.lean
@@ -2,7 +2,6 @@ import BlasterBenchmarks.UPLC.Builtins
 import BlasterBenchmarks.UPLC.CekValue
 import BlasterBenchmarks.UPLC.Examples.Utils
 import BlasterBenchmarks.UPLC.Examples.Onchain.ProcessSCOrder.ProcessSCOrder
-import BlasterBenchmarks.UPLC.PreProcess
 import BlasterBenchmarks.UPLC.Uplc
 import Solver.Command.Tactic
 
@@ -10,94 +9,14 @@ namespace Tests.Uplc.Onchain.ProcessSCOrder
 open Tests.Uplc.Onchain
 
 set_option warn.sorry false
--- TODO: complete proof
+-- STO8: Successful Selling Stablecoin Order
+
+-- Provable once subgoal splitting supported inherently in blaster
 theorem sto8 :
   ∀ (x : ProcessSCInput) (s : ComputeReserve),
     isSellSCOrder x →
     validOrderInput x →
-    resultToComputeReserve (fromHaltState $ prop_compiledProcessSCOrder x) = some s →
+    resultToComputeReserve (fromHaltState $ appliedProcessSCOrder x) = some s →
     validSellSC x s := by sorry
-    -- intro x s;
-    -- blaster (only-optimize: 1)
-    -- by_cases x.state.crN_SC = 0 <;>
-    -- by_cases x.state.crN_RC = 0
-    -- . blaster
-    -- . blaster
-    -- . blaster (only-optimize: 1); intros; repeat' constructor
-    --   . sorry
-    --   . by_cases x.orderRate < mkRatio x.state.crReserve x.state.crN_SC
-    --     . sorry
-    --     . sorry
-    --   . by_cases x.orderRate < mkRatio x.state.crReserve x.state.crN_SC <;> blaster
-    --   . blaster
-    --   . blaster (only-optimize: 1)
-    --     by_cases x.orderRate < mkRatio x.state.crReserve x.state.crN_SC
-    --     . let price := x.orderRate * x.scBaseFeeSSC
-    --       let adaForOrder := x.adaAtOrderUtxo - x.minAdaTransfer
-    --       let totalPrice := truncate $ fromInteger (-x.nbTokens) * price
-    --       let opFees := truncate $ fromInteger totalPrice * x.scOperatorFeeRatio
-    --       by_cases fromInteger opFees < fromInteger totalPrice * x.scOperatorFeeRatio
-    --       . by_cases 1 + opFees < x.scMinOperatorFee <;>
-    --         by_cases 1 + opFees < x.scMaxOperatorFee
-    --         . blaster
-    --         . blaster
-    --         . let totalPrice_code := -(truncate $ price * fromInteger x.nbTokens)
-    --           let opFees_code := truncate $ fromInteger totalPrice_code * x.scOperatorFeeRatio
-    --           by_cases fromInteger opFees_code < fromInteger totalPrice_code * x.scOperatorFeeRatio
-    --           . by_cases opFees < adaForOrder
-    --             . blaster
-    --             . by_cases zeroRatio < price <;>
-    --               by_cases price * x.scOperatorFeeRatio < zeroRatio <;>
-    --               by_cases adaForOrder < x.scMinOperatorFee
-    --               . blaster
-    --               . blaster
-    --               . blaster
-    --               . let n' := truncate $ fromInteger adaForOrder * (unsafeRecip $ price * x.scOperatorFeeRatio)
-    --                 let totalPrice' := truncate $ fromInteger (n' + 1) * price
-    --                 let opFees' := truncate $ fromInteger totalPrice' * x.scOperatorFeeRatio
-    --                 by_cases fromInteger opFees' < fromInteger totalPrice' * x.scOperatorFeeRatio
-    --                 . by_cases 1 + opFees' < x.scMinOperatorFee <;>
-    --                   by_cases 1 + opFees_code < x.scMinOperatorFee
-    --                   . blaster (timeout: 5)
-    --                   . by_cases opFees_code < adaForOrder <;>
-    --                     by_cases 1 + opFees_code < x.scMaxOperatorFee
-    --                     . blaster (timeout: 5)
-    --                     . blaster (timeout: 5)
-    --                     . sorry
-    --                     . blaster (timeout: 5)
-    --                   . blaster (timeout: 5)
-    --                   . by_cases 1 + opFees_code < x.scMaxOperatorFee <;>
-    --                     by_cases 1 + opFees' < x.scMaxOperatorFee
-    --                     . sorry
-    --                     . blaster (timeout: 5)
-    --                     . blaster (timeout: 5)
-    --                     . blaster (timeout: 5)
-    --                 . sorry
-    --               . blaster (timeout: 5)
-    --               . blaster (timeout: 5)
-    --               . blaster (timeout: 5)
-    --               . blaster (timeout: 5)
-    --           . blaster (timeout: 5)
-    --         . sorry
-    --       . sorry
-    --     . sorry
-    --   . by_cases x.orderRate < mkRatio x.state.crReserve x.state.crN_SC <;> blaster
-    --   . blaster (only-optimize: 1)
-    --     by_cases x.orderRate < mkRatio x.state.crReserve x.state.crN_SC
-    --     . let totalPrice := truncate $ fromInteger (-x.nbTokens) * (x.orderRate * x.scBaseFeeSSC)
-    --       let opFees := truncate $ fromInteger totalPrice * x.scOperatorFeeRatio
-    --       by_cases fromInteger opFees < fromInteger totalPrice * x.scOperatorFeeRatio
-    --       . blaster
-    --       . blaster (random-seed: 3)
-    --     . let r_price := mkRatio x.state.crReserve x.state.crN_SC
-    --       let totalPrice := truncate $ fromInteger (-x.nbTokens) * (r_price * x.scBaseFeeSSC)
-    --       let opFees := truncate $ fromInteger totalPrice * x.scOperatorFeeRatio
-    --       by_cases fromInteger opFees < fromInteger totalPrice * x.scOperatorFeeRatio
-    --       . blaster (random-seed: 2)
-    --       . by_cases r_price * x.scBaseFeeSSC * x.scOperatorFeeRatio < zeroRatio <;> blaster
-    -- . sorry
-
--- NOTE: Remove solver options once subgoal splitting is supported
-#solve (timeout: 2) (solve-result: 2) [sto8]
 
 end Tests.Uplc.Onchain.ProcessSCOrder
